ds_abs0/abs_relScript.sml
@@ -1,5 +1,5 @@
 open HolKernel bossLib boolLib Parse;
-open ds_abs0_stateTheory ds_abs1_stateTheory;
+open ds_abs0_stateTheory ds_abs1_stateTheory ref_relTheory;
 
 val _ = new_theory "abs_rel"
 
@@ -95,5 +95,16 @@ EL (ds_abs1.ds_abs1_tx.tx_cur_length - 1) (ds_abs1.ds_abs1_tx.tx_data_buffer)) /
 (ds_abs0.state = abs0_xfer_done ==> ds_abs1.spi_abs1.RX_SHIFT_REG = ds_abs0.ds_abs0_xfer.xfer_RSR) /\
 (ds_abs1.state = abs1_xfer_exchange ==> ds_abs1.spi_abs1.TX_SHIFT_REG = 
 EL (ds_abs1.ds_abs1_xfer.xfer_cur_length - 1) (ds_abs1.ds_abs1_xfer.xfer_dataOUT_buffer)))`
+
+(* abs0_comb_rel: ds_abs0_state -> (driver_state * spi_state) -> bool *)
+val abs0_comb_rel_def = Define `
+abs0_comb_rel (ds_abs0:ds_abs0_state) (dr:driver_state, spi:spi_state) = 
+(?ds_abs1:ds_abs1_state. abs_rel ds_abs0 ds_abs1 /\ ref_rel ds_abs1 (dr,spi))`
+
+(* global abs0_comb_rel:
+(ds_abs0_state * ds_abs0_state) -> (driver_state * spi_state * driver_state * spi_state) -> bool *)
+val global_abs0_comb_rel_def = Define `
+global_abs0_comb_rel (d0, d1) (dr0, spi0, dr1, spi1) =
+(abs0_comb_rel d0 (dr0,spi0) /\ abs0_comb_rel d1 (dr1,spi1))`
 
 val _ = export_theory();
