general_thm/abs0_comb_weak_bisimulation.sml
@@ -3,10 +3,7 @@ open ds_abs0_stateTheory abs_relTheory driver_stateTheory SPI_stateTheory ds_abs
 
 val _ = new_theory "abs0_comb_weak_bisimulation";
 
-val abs0_comb_rel_def = Define `
-abs0_comb_rel (ds_abs0:ds_abs0_state) (dr:driver_state, spi:spi_state) = 
-(?ds_abs1:ds_abs1_state. abs_rel ds_abs0 ds_abs1 /\ ref_rel ds_abs1 (dr,spi))`
-
+(* some lemmas about n_tau_tr *)
 val n_tau_tr_last = store_thm ("n_tau_tr_last",
 ``!tr s s' s'' lbl n.
 n_tau_tr n tr s tau s'' /\ tr s'' lbl s' ==>
@@ -63,6 +60,223 @@ Q.EXISTS_TAC `spi'` >>
 rw [] >>
 METIS_TAC [n_tau_tr_plus]);
 
+val n_tau_tr_local_global_tr_first = store_thm("n_tau_tr_local_global_tr_first",
+``!n dr0 spi0 dr1 spi1 dr0' spi0' lbl.
+n_tau_tr n local_tr (dr0,spi0) lbl (dr0',spi0') /\
+(!d. lbl <> TX d) /\ (!d. lbl <> RX d) /\ (!d0 d1. lbl <> XFER d0 d1) ==>
+n_tau_tr n global_tr (dr0,spi0,dr1,spi1) tau (dr0',spi0',dr1,spi1)``,
+Induct_on `n` >>
+rw [n_tau_tr_def] >-
+(rw [global_tr_cases] >>
+fs [local_tr_cases] >>
+METIS_TAC []) >>
+Cases_on `s''` >>
+Q.EXISTS_TAC `(q,r,dr1,spi1)` >>
+rw [global_tr_cases] >>
+METIS_TAC []);
+
+val n_tau_tr_local_global_tr_second = store_thm("n_tau_tr_local_global_tr_second",
+``!n dr0 spi0 dr1 spi1 dr1' spi1' lbl.
+n_tau_tr n local_tr (dr1,spi1) lbl (dr1',spi1') /\
+(!d. lbl <> TX d) /\ (!d. lbl <> RX d) /\ (!d0 d1. lbl <> XFER d0 d1) ==>
+n_tau_tr n global_tr (dr0,spi0,dr1,spi1) tau (dr0,spi0,dr1',spi1')``,
+Induct_on `n` >>
+rw [n_tau_tr_def] >-
+(rw [global_tr_cases] >>
+fs [local_tr_cases] >>
+METIS_TAC []) >>
+Cases_on `s''` >>
+Q.EXISTS_TAC `(dr0,spi0,q,r)` >>
+rw [global_tr_cases] >>
+METIS_TAC []);
+
+val d0_TX_d1_RX_n_tau_tr = store_thm("d0_TX_d1_RX_n_tau_tr",
+``!n dr0 spi0 dr0' spi0' dr1 spi1 dr1' spi1' data.
+n_tau_tr n local_tr (dr1,spi1) (RX data) (dr1',spi1') /\
+local_tr (dr0,spi0) (TX data) (dr0',spi0') ==>
+n_tau_tr n global_tr (dr0,spi0,dr1,spi1) tau (dr0',spi0',dr1',spi1')``,
+Induct_on `n` >>
+rw [n_tau_tr_def] >-
+(rw [global_tr_cases] >>
+METIS_TAC []) >>
+Cases_on `s''` >>
+Q.EXISTS_TAC `(dr0,spi0,q,r)` >>
+rw [global_tr_cases] >>
+METIS_TAC []);
+
+val d1_TX_d0_RX_n_tau_tr = store_thm("d1_TX_d0_RX_n_tau_tr",
+``!n dr0 spi0 dr0' spi0' dr1 spi1 dr1' spi1' data.
+n_tau_tr n local_tr (dr0,spi0) (RX data) (dr0',spi0') /\
+local_tr (dr1,spi1) (TX data) (dr1',spi1') ==>
+n_tau_tr n global_tr (dr0,spi0,dr1,spi1) tau (dr0',spi0',dr1',spi1')``,
+Induct_on `n` >>
+rw [n_tau_tr_def] >-
+(rw [global_tr_cases] >>
+METIS_TAC []) >>
+Cases_on `s''` >>
+Q.EXISTS_TAC `(q,r,dr1,spi1)` >>
+rw [global_tr_cases] >>
+METIS_TAC []);
+
+val d0_TX_n_tau_tr_d1_RX = store_thm("d0_TX_n_tau_tr_d1_RX",
+``!n dr0 spi0 dr0' spi0' dr1 spi1 dr1' spi1' data.
+local_tr (dr1,spi1) (RX data) (dr1',spi1') /\
+n_tau_tr n local_tr (dr0,spi0) (TX data) (dr0',spi0') ==>
+n_tau_tr n global_tr (dr0,spi0,dr1,spi1) tau (dr0',spi0',dr1',spi1')``,
+Induct_on `n` >>
+rw [n_tau_tr_def] >-
+(rw [global_tr_cases] >>
+METIS_TAC []) >>
+Cases_on `s''` >>
+Q.EXISTS_TAC `(q,r,dr1,spi1)` >>
+rw [global_tr_cases] >>
+METIS_TAC []);
+
+val d1_TX_n_tau_tr_d0_RX = store_thm("d1_TX_n_tau_tr_d0_RX",
+``!n dr0 spi0 dr0' spi0' dr1 spi1 dr1' spi1' data.
+n_tau_tr n local_tr (dr1,spi1) (TX data) (dr1',spi1') /\
+local_tr (dr0,spi0) (RX data) (dr0',spi0') ==>
+n_tau_tr n global_tr (dr0,spi0,dr1,spi1) tau (dr0',spi0',dr1',spi1')``,
+Induct_on `n` >>
+rw [n_tau_tr_def] >-
+(rw [global_tr_cases] >>
+METIS_TAC []) >>
+Cases_on `s''` >>
+Q.EXISTS_TAC `(dr0,spi0,q,r)` >>
+rw [global_tr_cases] >>
+METIS_TAC []);
+
+val d0_TX_d1_RX_n_plus_n' = store_thm("d0_TX_d1_RX_n_plus_n'",
+``!n n' dr0 spi0 dr0' spi0' dr1 spi1 dr1' spi1' data.
+n_tau_tr n local_tr (dr1,spi1) (RX data) (dr1',spi1') /\
+n_tau_tr n' local_tr (dr0,spi0) (TX data) (dr0',spi0') ==>
+n_tau_tr (n + n') global_tr (dr0,spi0,dr1,spi1) tau (dr0',spi0',dr1',spi1')``,
+Induct_on `n` >>
+Induct_on `n'` >>
+rw [n_tau_tr_def] >-
+(rw [global_tr_cases] >>
+METIS_TAC []) >-
+(Cases_on `s''` >>
+Q.EXISTS_TAC `(q,r,dr1,spi1)` >>
+rw [global_tr_cases] >>
+fs [n_tau_tr_def] >>
+METIS_TAC []) >-
+(Cases_on `s''` >>
+Q.EXISTS_TAC `(dr0,spi0,q,r)` >>
+rw [global_tr_cases] >>
+`!dr0 spi0 dr0' spi0' dr1 spi1 dr1' spi1' data.
+n_tau_tr n local_tr (dr1,spi1) (RX data) (dr1',spi1') /\
+n_tau_tr 0 local_tr (dr0,spi0) (TX data) (dr0',spi0') ==>
+n_tau_tr (n + 0) global_tr (dr0,spi0,dr1,spi1) tau (dr0',spi0',dr1',spi1')` by METIS_TAC [] >>
+fs [n_tau_tr_def] >>
+METIS_TAC []) >>
+`SUC n + SUC n' = SUC (SUC (n + n'))` by rw [] >>
+rw [n_tau_tr_def] >>
+Cases_on `s''` >>
+Cases_on `s'''` >>
+Q.EXISTS_TAC `(q',r',dr1,spi1)` >>
+rw [global_tr_cases] >>
+Q.EXISTS_TAC `(q',r',q,r)` >> 
+fs [] >>
+METIS_TAC []);
+
+val d1_TX_d0_RX_n_plus_n' = store_thm("d0_TX_d1_RX_n_plus_n'",
+``!n n' dr0 spi0 dr0' spi0' dr1 spi1 dr1' spi1' data.
+n_tau_tr n local_tr (dr1,spi1) (TX data) (dr1',spi1') /\
+n_tau_tr n' local_tr (dr0,spi0) (RX data) (dr0',spi0') ==>
+n_tau_tr (n + n') global_tr (dr0,spi0,dr1,spi1) tau (dr0',spi0',dr1',spi1')``,
+Induct_on `n` >>
+Induct_on `n'` >>
+rw [n_tau_tr_def] >-
+(rw [global_tr_cases] >>
+METIS_TAC []) >-
+(Cases_on `s''` >>
+Q.EXISTS_TAC `(q,r,dr1,spi1)` >>
+rw [global_tr_cases] >>
+fs [n_tau_tr_def] >>
+METIS_TAC []) >-
+(Cases_on `s''` >>
+Q.EXISTS_TAC `(dr0,spi0,q,r)` >>
+rw [global_tr_cases] >>
+`!dr0 spi0 dr0' spi0' dr1 spi1 dr1' spi1' data.
+n_tau_tr n local_tr (dr1,spi1) (TX data) (dr1',spi1') /\
+n_tau_tr 0 local_tr (dr0,spi0) (RX data) (dr0',spi0') ==>
+n_tau_tr (n + 0) global_tr (dr0,spi0,dr1,spi1) tau (dr0',spi0',dr1',spi1')` by METIS_TAC [] >>
+fs [n_tau_tr_def] >>
+METIS_TAC []) >>
+`SUC n + SUC n' = SUC (SUC (n + n'))` by rw [] >>
+rw [n_tau_tr_def] >>
+Cases_on `s''` >>
+Cases_on `s'''` >>
+Q.EXISTS_TAC `(q',r',dr1,spi1)` >>
+rw [global_tr_cases] >>
+Q.EXISTS_TAC `(q',r',q,r)` >> 
+fs [] >>
+METIS_TAC []);
+
+val XFER_d0_d1_n_tau_tr = store_thm("XFER_d0_d1_n_tau_tr",
+``!n dr0 spi0 dr0' spi0' dr1 spi1 dr1' spi1' dataI dataO.
+n_tau_tr n local_tr (dr1,spi1) (XFER dataO dataI) (dr1',spi1') /\
+local_tr (dr0,spi0) (XFER dataI dataO) (dr0',spi0') ==>
+n_tau_tr n global_tr (dr0,spi0,dr1,spi1) tau (dr0',spi0',dr1',spi1')``,
+Induct_on `n` >>
+rw [n_tau_tr_def] >-
+(rw [global_tr_cases] >>
+METIS_TAC []) >>
+Cases_on `s''` >>
+Q.EXISTS_TAC `(dr0,spi0,q,r)` >>
+rw [global_tr_cases] >>
+METIS_TAC []);
+
+val XFER_d0_n_tau_tr_d1 = store_thm("XFER_d0_n_tau_tr_d1",
+``!n dr0 spi0 dr0' spi0' dr1 spi1 dr1' spi1' dataI dataO.
+local_tr (dr1,spi1) (XFER dataO dataI) (dr1',spi1') /\
+n_tau_tr n local_tr (dr0,spi0) (XFER dataI dataO) (dr0',spi0') ==>
+n_tau_tr n global_tr (dr0,spi0,dr1,spi1) tau (dr0',spi0',dr1',spi1')``,
+Induct_on `n` >>
+rw [n_tau_tr_def] >-
+(rw [global_tr_cases] >>
+METIS_TAC []) >>
+Cases_on `s''` >>
+Q.EXISTS_TAC `(q,r,dr1,spi1)` >>
+rw [global_tr_cases] >>
+METIS_TAC []);
+
+val XFER_d0_d1_n_plus_n' = store_thm("XFER_d0_d1_n_plus_n'",
+``!n n' dr0 spi0 dr0' spi0' dr1 spi1 dr1' spi1' dataI dataO.
+n_tau_tr n local_tr (dr1,spi1) (XFER dataO dataI) (dr1',spi1') /\
+n_tau_tr n' local_tr (dr0,spi0) (XFER dataI dataO) (dr0',spi0') ==>
+n_tau_tr (n + n') global_tr (dr0,spi0,dr1,spi1) tau (dr0',spi0',dr1',spi1')``,
+Induct_on `n` >>
+Induct_on `n'` >>
+rw [n_tau_tr_def] >-
+(rw [global_tr_cases] >>
+METIS_TAC []) >-
+(Cases_on `s''` >>
+Q.EXISTS_TAC `(q,r,dr1,spi1)` >>
+rw [global_tr_cases] >>
+fs [n_tau_tr_def] >>
+METIS_TAC []) >-
+(Cases_on `s''` >>
+Q.EXISTS_TAC `(dr0,spi0,q,r)` >>
+rw [global_tr_cases] >>
+`!dr0 spi0 dr0' spi0' dr1 spi1 dr1' spi1' dataI dataO.
+n_tau_tr n local_tr (dr1,spi1) (XFER dataO dataI) (dr1',spi1') /\
+n_tau_tr 0 local_tr (dr0,spi0) (XFER dataI dataO) (dr0',spi0') ==>
+n_tau_tr (n + 0) global_tr (dr0,spi0,dr1,spi1) tau (dr0',spi0',dr1',spi1')` by METIS_TAC [] >>
+fs [n_tau_tr_def] >>
+METIS_TAC []) >>
+`SUC n + SUC n' = SUC (SUC (n + n'))` by rw [] >>
+rw [n_tau_tr_def] >>
+Cases_on `s''` >>
+Cases_on `s'''` >>
+Q.EXISTS_TAC `(q',r',dr1,spi1)` >>
+rw [global_tr_cases] >>
+Q.EXISTS_TAC `(q',r',q,r)` >> 
+fs [] >>
+METIS_TAC []);
+
+(* weak bisimulation of the abs0 and concrete models *)
 val weak_bisimulation_abs0_comb = store_thm("weak_bisimulation_abs0_comb",
 ``weak_bisim abs0_comb_rel ds_abs0_tr local_tr``,
 `weak_bisim abs_rel ds_abs0_tr ds_abs1_tr` by rw [weak_bisimulation_abs0_abs1] >>
@@ -104,5 +318,332 @@ Q.EXISTS_TAC `ds_abs1` >> rw []) >>
 Q.EXISTS_TAC `s1'` >>
 rw [abs0_comb_rel_def] >>
 Q.EXISTS_TAC `ds_abs1'` >> rw []);
+
+(* weak bisimulation for the global transition relations of abs0 and concrete models *)
+val weak_bisimulation_global_abs0_comb = store_thm("weak_bisimulation_global_abs0_comb",
+``weak_bisim global_abs0_comb_rel abs0_global_tr global_tr``,
+`weak_bisim abs0_comb_rel ds_abs0_tr local_tr` by rw [weak_bisimulation_abs0_comb] >>
+fs [weak_bisim_def] >>
+rw [] >>
+Cases_on `s1` >>
+Cases_on `s2` >>
+Cases_on `r'` >>
+Cases_on `r''` >- 
+((* (dr0',spi0',dr1',spi1') exists *)
+fs [global_abs0_comb_rel_def, abs0_global_tr_cases] >|
+[`?s2'. weak_tr local_tr (q',q'') call_init s2' /\ abs0_comb_rel d0' s2'` by METIS_TAC [] >>
+Cases_on `s2'` >>
+Q.EXISTS_TAC `(q'''',r'',q''',r')` >>
+fs [global_abs0_comb_rel_def, weak_tr_def] >-
+(DISJ1_TAC >>
+rw [global_tr_cases]) >>
+REPEAT DISJ2_TAC >>
+Q.EXISTS_TAC `n` >>
+`(!d. call_init <> TX d) /\
+(!d. call_init <> RX d) /\
+(!d0 d1. call_init <> XFER d0 d1)` by rw [] >>
+METIS_TAC [n_tau_tr_local_global_tr_first],
+`?s2'. weak_tr local_tr (q''',r') call_init s2' /\ abs0_comb_rel d1' s2'` by METIS_TAC [] >>
+Cases_on `s2'` >>
+Q.EXISTS_TAC `(q',q'',q'''',r'')` >>
+fs [global_abs0_comb_rel_def, weak_tr_def] >-
+(DISJ1_TAC >>
+rw [global_tr_cases]) >>
+REPEAT DISJ2_TAC >>
+Q.EXISTS_TAC `n` >>
+`(!d. call_init <> TX d) /\
+(!d. call_init <> RX d) /\
+(!d0 d1. call_init <> XFER d0 d1)` by rw [] >>
+METIS_TAC [n_tau_tr_local_global_tr_second],
+`?s2'. weak_tr local_tr (q',q'') (call_tx buffer) s2' /\ abs0_comb_rel d0' s2'` by METIS_TAC [] >>
+Cases_on `s2'` >>
+Q.EXISTS_TAC `(q'''',r'',q''',r')` >>
+fs [global_abs0_comb_rel_def, weak_tr_def] >-
+(DISJ1_TAC >>
+rw [global_tr_cases] >>
+METIS_TAC []) >>
+REPEAT DISJ2_TAC >>
+Q.EXISTS_TAC `n` >>
+`(!d. call_tx buffer <> TX d) /\
+(!d. call_tx buffer <> RX d) /\
+(!d0 d1. call_tx buffer <> XFER d0 d1)` by rw [] >>
+METIS_TAC [n_tau_tr_local_global_tr_first],
+`?s2'. weak_tr local_tr (q''',r') (call_tx buffer) s2' /\ abs0_comb_rel d1' s2'` by METIS_TAC [] >>
+Cases_on `s2'` >>
+Q.EXISTS_TAC `(q',q'',q'''',r'')` >>
+fs [global_abs0_comb_rel_def, weak_tr_def] >-
+(DISJ1_TAC >>
+rw [global_tr_cases] >>
+METIS_TAC []) >>
+REPEAT DISJ2_TAC >>
+Q.EXISTS_TAC `n` >>
+`(!d. call_tx buffer <> TX d) /\
+(!d. call_tx buffer <> RX d) /\
+(!d0 d1. call_tx buffer <> XFER d0 d1)` by rw [] >>
+METIS_TAC [n_tau_tr_local_global_tr_second],
+`?s2'. weak_tr local_tr (q',q'') (call_rx l) s2' /\ abs0_comb_rel d0' s2'` by METIS_TAC [] >>
+Cases_on `s2'` >>
+Q.EXISTS_TAC `(q'''',r'',q''',r')` >>
+fs [global_abs0_comb_rel_def, weak_tr_def] >-
+(DISJ1_TAC >>
+rw [global_tr_cases] >>
+METIS_TAC []) >>
+REPEAT DISJ2_TAC >>
+Q.EXISTS_TAC `n` >>
+`(!d. call_rx l <> TX d) /\
+(!d. call_rx l <> RX d) /\
+(!d0 d1. call_rx l <> XFER d0 d1)` by rw [] >>
+METIS_TAC [n_tau_tr_local_global_tr_first],
+`?s2'. weak_tr local_tr (q''',r') (call_rx l) s2' /\ abs0_comb_rel d1' s2'` by METIS_TAC [] >>
+Cases_on `s2'` >>
+Q.EXISTS_TAC `(q',q'',q'''',r'')` >>
+fs [global_abs0_comb_rel_def, weak_tr_def] >-
+(DISJ1_TAC >>
+rw [global_tr_cases] >>
+METIS_TAC []) >>
+REPEAT DISJ2_TAC >>
+Q.EXISTS_TAC `n` >>
+`(!d. call_rx l <> TX d) /\
+(!d. call_rx l <> RX d) /\
+(!d0 d1. call_rx l <> XFER d0 d1)` by rw [] >>
+METIS_TAC [n_tau_tr_local_global_tr_second],
+`?s2'. weak_tr local_tr (q',q'') (call_xfer buffer0) s2' /\ abs0_comb_rel d0' s2'` by METIS_TAC [] >>
+Cases_on `s2'` >>
+Q.EXISTS_TAC `(q'''',r'',q''',r')` >>
+fs [global_abs0_comb_rel_def, weak_tr_def] >-
+(DISJ1_TAC >>
+rw [global_tr_cases] >>
+METIS_TAC []) >>
+REPEAT DISJ2_TAC >>
+Q.EXISTS_TAC `n` >>
+`(!d. call_xfer buffer0 <> TX d) /\
+(!d. call_xfer buffer0 <> RX d) /\
+(!d0 d1. call_xfer buffer0 <> XFER d0 d1)` by rw [] >>
+METIS_TAC [n_tau_tr_local_global_tr_first],
+`?s2'. weak_tr local_tr (q''',r') (call_xfer buffer1) s2' /\ abs0_comb_rel d1' s2'` by METIS_TAC [] >>
+Cases_on `s2'` >>
+Q.EXISTS_TAC `(q',q'',q'''',r'')` >>
+fs [global_abs0_comb_rel_def, weak_tr_def] >-
+(DISJ1_TAC >>
+rw [global_tr_cases] >>
+METIS_TAC []) >>
+REPEAT DISJ2_TAC >>
+Q.EXISTS_TAC `n` >>
+`(!d. call_xfer buffer1 <> TX d) /\
+(!d. call_xfer buffer1 <> RX d) /\
+(!d0 d1. call_xfer buffer1 <> XFER d0 d1)` by rw [] >>
+METIS_TAC [n_tau_tr_local_global_tr_second],
+`?s2'. weak_tr local_tr (q',q'') tau s2' /\ abs0_comb_rel d0' s2'` by METIS_TAC [] >>
+Cases_on `s2'` >>
+Q.EXISTS_TAC `(q'''',r'',q''',r')` >>
+fs [global_abs0_comb_rel_def, weak_tr_def] >-
+(DISJ1_TAC >>
+rw [global_tr_cases] >>
+METIS_TAC []) >>
+REPEAT DISJ2_TAC >>
+Q.EXISTS_TAC `n` >>
+`(!d. tau <> TX d) /\
+(!d. tau <> RX d) /\
+(!d0 d1. tau <> XFER d0 d1)` by rw [] >>
+METIS_TAC [n_tau_tr_local_global_tr_first],
+`?s2'. weak_tr local_tr (q''',r') tau s2' /\ abs0_comb_rel d1' s2'` by METIS_TAC [] >>
+Cases_on `s2'` >>
+Q.EXISTS_TAC `(q',q'',q'''',r'')` >>
+fs [global_abs0_comb_rel_def, weak_tr_def] >-
+(DISJ1_TAC >>
+rw [global_tr_cases] >>
+METIS_TAC []) >>
+REPEAT DISJ2_TAC >>
+Q.EXISTS_TAC `n` >>
+`(!d. tau <> TX d) /\
+(!d. tau <> RX d) /\
+(!d0 d1. tau <> XFER d0 d1)` by rw [] >>
+METIS_TAC [n_tau_tr_local_global_tr_second],
+`?s2'. weak_tr local_tr (q',q'') (TX data) s2' /\ abs0_comb_rel d0' s2'` by METIS_TAC [] >>
+`?s2''. weak_tr local_tr (q''',r') (RX data) s2'' /\ abs0_comb_rel d1' s2''` by METIS_TAC [] >>
+Cases_on `s2'` >> Cases_on `s2''` >>
+Q.EXISTS_TAC `(q'''',r'',q''''',r''')` >>
+fs [global_abs0_comb_rel_def, weak_tr_def] >-
+(DISJ1_TAC >>
+rw [global_tr_cases] >>
+METIS_TAC []) >>
+REPEAT DISJ2_TAC >|
+[Q.EXISTS_TAC `n` >> METIS_TAC [d0_TX_d1_RX_n_tau_tr],
+ Q.EXISTS_TAC `n` >> METIS_TAC [d0_TX_n_tau_tr_d1_RX],
+ Q.EXISTS_TAC `n' + n` >> METIS_TAC [d0_TX_d1_RX_n_plus_n']],
+`?s2'. weak_tr local_tr (q',q'') (RX data) s2' /\ abs0_comb_rel d0' s2'` by METIS_TAC [] >>
+`?s2''. weak_tr local_tr (q''',r') (TX data) s2'' /\ abs0_comb_rel d1' s2''` by METIS_TAC [] >>
+Cases_on `s2'` >> Cases_on `s2''` >>
+Q.EXISTS_TAC `(q'''',r'',q''''',r''')` >>
+fs [global_abs0_comb_rel_def, weak_tr_def] >-
+(DISJ1_TAC >>
+rw [global_tr_cases] >>
+METIS_TAC []) >>
+REPEAT DISJ2_TAC >|
+[Q.EXISTS_TAC `n` >> METIS_TAC [d1_TX_n_tau_tr_d0_RX],
+ Q.EXISTS_TAC `n` >> METIS_TAC [d1_TX_d0_RX_n_tau_tr],
+ Q.EXISTS_TAC `n' + n` >> METIS_TAC [d1_TX_d0_RX_n_plus_n']],
+`?s2'. weak_tr local_tr (q',q'') (XFER dataI dataO) s2' /\ abs0_comb_rel d0' s2'` by METIS_TAC [] >>
+`?s2''. weak_tr local_tr (q''',r') (XFER dataO dataI) s2'' /\ abs0_comb_rel d1' s2''` by METIS_TAC [] >>
+Cases_on `s2'` >> Cases_on `s2''` >>
+Q.EXISTS_TAC `(q'''',r'',q''''',r''')` >>
+fs [global_abs0_comb_rel_def, weak_tr_def] >-
+(DISJ1_TAC >>
+rw [global_tr_cases] >>
+METIS_TAC []) >>
+REPEAT DISJ2_TAC >|
+[Q.EXISTS_TAC `n` >> METIS_TAC [XFER_d0_d1_n_tau_tr],
+ Q.EXISTS_TAC `n` >> METIS_TAC [XFER_d0_n_tau_tr_d1],
+ Q.EXISTS_TAC `n' + n` >> METIS_TAC [XFER_d0_d1_n_plus_n']]]) >>
+(* (d0',d1') exists *)
+fs [global_abs0_comb_rel_def, abs0_comb_rel_def, global_tr_cases] >|
+[`call_init <> tau` by rw [] >>
+`?ds_abs1''. (ds_abs1_tr ds_abs1 call_init ds_abs1'') /\ (ref_rel ds_abs1'' (dr1', spi1'))` by METIS_TAC [comb_abs1_weak_simulation_lbl_not_tau] >>
+`?ds_abs0'. (ds_abs0_tr q call_init ds_abs0') /\ (abs_rel ds_abs0' ds_abs1'')` by METIS_TAC [abs1_abs0_weak_simulation] >>
+Q.EXISTS_TAC `(ds_abs0',r)` >>
+rw [global_abs0_comb_rel_def, abs0_comb_rel_def, weak_tr_def] >|
+[DISJ1_TAC >>
+rw [abs0_global_tr_cases],
+Q.EXISTS_TAC `ds_abs1''` >> rw [],
+Q.EXISTS_TAC `ds_abs1'` >> rw []],
+`call_init <> tau` by rw [] >>
+`?ds_abs1''. (ds_abs1_tr ds_abs1' call_init ds_abs1'') /\ (ref_rel ds_abs1'' (dr2', spi2'))` by METIS_TAC [comb_abs1_weak_simulation_lbl_not_tau] >>
+`?ds_abs0'. (ds_abs0_tr r call_init ds_abs0') /\ (abs_rel ds_abs0' ds_abs1'')` by METIS_TAC [abs1_abs0_weak_simulation] >>
+Q.EXISTS_TAC `(q,ds_abs0')` >>
+rw [global_abs0_comb_rel_def, abs0_comb_rel_def, weak_tr_def] >|
+[DISJ1_TAC >>
+rw [abs0_global_tr_cases],
+Q.EXISTS_TAC `ds_abs1` >> rw [],
+Q.EXISTS_TAC `ds_abs1''` >> rw []],
+`call_tx buffer <> tau` by rw [] >>
+`?ds_abs1''. (ds_abs1_tr ds_abs1 (call_tx buffer) ds_abs1'') /\ (ref_rel ds_abs1'' (dr1', spi1'))` by METIS_TAC [comb_abs1_weak_simulation_lbl_not_tau] >>
+`?ds_abs0'. (ds_abs0_tr q (call_tx buffer) ds_abs0') /\ (abs_rel ds_abs0' ds_abs1'')` by METIS_TAC [abs1_abs0_weak_simulation] >>
+Q.EXISTS_TAC `(ds_abs0',r)` >>
+rw [global_abs0_comb_rel_def, abs0_comb_rel_def, weak_tr_def] >|
+[DISJ1_TAC >>
+rw [abs0_global_tr_cases] >>
+METIS_TAC [],
+Q.EXISTS_TAC `ds_abs1''` >> rw [],
+Q.EXISTS_TAC `ds_abs1'` >> rw []],
+`call_tx buffer <> tau` by rw [] >>
+`?ds_abs1''. (ds_abs1_tr ds_abs1' (call_tx buffer) ds_abs1'') /\ (ref_rel ds_abs1'' (dr2', spi2'))` by METIS_TAC [comb_abs1_weak_simulation_lbl_not_tau] >>
+`?ds_abs0'. (ds_abs0_tr r (call_tx buffer) ds_abs0') /\ (abs_rel ds_abs0' ds_abs1'')` by METIS_TAC [abs1_abs0_weak_simulation] >>
+Q.EXISTS_TAC `(q,ds_abs0')` >>
+rw [global_abs0_comb_rel_def, abs0_comb_rel_def, weak_tr_def] >|
+[DISJ1_TAC >>
+rw [abs0_global_tr_cases] >>
+METIS_TAC [],
+Q.EXISTS_TAC `ds_abs1` >> rw [],
+Q.EXISTS_TAC `ds_abs1''` >> rw []],
+`call_rx length <> tau` by rw [] >>
+`?ds_abs1''. (ds_abs1_tr ds_abs1 (call_rx length) ds_abs1'') /\ (ref_rel ds_abs1'' (dr1', spi1'))` by METIS_TAC [comb_abs1_weak_simulation_lbl_not_tau] >>
+`?ds_abs0'. (ds_abs0_tr q (call_rx length) ds_abs0') /\ (abs_rel ds_abs0' ds_abs1'')` by METIS_TAC [abs1_abs0_weak_simulation] >>
+Q.EXISTS_TAC `(ds_abs0',r)` >>
+rw [global_abs0_comb_rel_def, abs0_comb_rel_def, weak_tr_def] >|
+[DISJ1_TAC >>
+rw [abs0_global_tr_cases] >>
+METIS_TAC [],
+Q.EXISTS_TAC `ds_abs1''` >> rw [],
+Q.EXISTS_TAC `ds_abs1'` >> rw []],
+`call_rx length <> tau` by rw [] >>
+`?ds_abs1''. (ds_abs1_tr ds_abs1' (call_rx length) ds_abs1'') /\ (ref_rel ds_abs1'' (dr2', spi2'))` by METIS_TAC [comb_abs1_weak_simulation_lbl_not_tau] >>
+`?ds_abs0'. (ds_abs0_tr r (call_rx length) ds_abs0') /\ (abs_rel ds_abs0' ds_abs1'')` by METIS_TAC [abs1_abs0_weak_simulation] >>
+Q.EXISTS_TAC `(q,ds_abs0')` >>
+rw [global_abs0_comb_rel_def, abs0_comb_rel_def, weak_tr_def] >|
+[DISJ1_TAC >>
+rw [abs0_global_tr_cases] >>
+METIS_TAC [],
+Q.EXISTS_TAC `ds_abs1` >> rw [],
+Q.EXISTS_TAC `ds_abs1''` >> rw []],
+`call_xfer buffer <> tau` by rw [] >>
+`?ds_abs1''. (ds_abs1_tr ds_abs1 (call_xfer buffer) ds_abs1'') /\ (ref_rel ds_abs1'' (dr1', spi1'))` by METIS_TAC [comb_abs1_weak_simulation_lbl_not_tau] >>
+`?ds_abs0'. (ds_abs0_tr q (call_xfer buffer) ds_abs0') /\ (abs_rel ds_abs0' ds_abs1'')` by METIS_TAC [abs1_abs0_weak_simulation] >>
+Q.EXISTS_TAC `(ds_abs0',r)` >>
+rw [global_abs0_comb_rel_def, abs0_comb_rel_def, weak_tr_def] >|
+[DISJ1_TAC >>
+rw [abs0_global_tr_cases] >>
+METIS_TAC [],
+Q.EXISTS_TAC `ds_abs1''` >> rw [],
+Q.EXISTS_TAC `ds_abs1'` >> rw []],
+`call_xfer buffer <> tau` by rw [] >>
+`?ds_abs1''. (ds_abs1_tr ds_abs1' (call_xfer buffer) ds_abs1'') /\ (ref_rel ds_abs1'' (dr2', spi2'))` by METIS_TAC [comb_abs1_weak_simulation_lbl_not_tau] >>
+`?ds_abs0'. (ds_abs0_tr r (call_xfer buffer) ds_abs0') /\ (abs_rel ds_abs0' ds_abs1'')` by METIS_TAC [abs1_abs0_weak_simulation] >>
+Q.EXISTS_TAC `(q,ds_abs0')` >>
+rw [global_abs0_comb_rel_def, abs0_comb_rel_def, weak_tr_def] >|
+[DISJ1_TAC >>
+rw [abs0_global_tr_cases] >>
+METIS_TAC [],
+Q.EXISTS_TAC `ds_abs1` >> rw [],
+Q.EXISTS_TAC `ds_abs1''` >> rw []],
+`ref_rel ds_abs1 (dr1',spi1') \/
+?ds_abs1''. ds_abs1_tr ds_abs1 tau ds_abs1'' /\ ref_rel ds_abs1'' (dr1',spi1')` by METIS_TAC [comb_abs1_weak_simulation_tau] >-
+(Q.EXISTS_TAC `(q,r)` >>
+rw [global_abs0_comb_rel_def, abs0_comb_rel_def, weak_tr_def] >>
+METIS_TAC []) >>
+`abs_rel q ds_abs1'' \/
+?ds_abs0'. ds_abs0_tr q tau ds_abs0' /\ abs_rel ds_abs0' ds_abs1''` by METIS_TAC [abs1_abs0_weak_simulation] >-
+(Q.EXISTS_TAC `(q,r)` >>
+rw [global_abs0_comb_rel_def, abs0_comb_rel_def, weak_tr_def] >>
+METIS_TAC []) >>
+Q.EXISTS_TAC `(ds_abs0',r)` >>
+rw [global_abs0_comb_rel_def, abs0_comb_rel_def, weak_tr_def] >|
+[DISJ1_TAC >>
+rw [abs0_global_tr_cases] >>
+METIS_TAC [],
+Q.EXISTS_TAC `ds_abs1''` >> rw [],
+Q.EXISTS_TAC `ds_abs1'` >> rw []],
+`ref_rel ds_abs1' (dr2',spi2') \/
+?ds_abs1''. ds_abs1_tr ds_abs1' tau ds_abs1'' /\ ref_rel ds_abs1'' (dr2',spi2')` by METIS_TAC [comb_abs1_weak_simulation_tau] >-
+(Q.EXISTS_TAC `(q,r)` >>
+rw [global_abs0_comb_rel_def, abs0_comb_rel_def, weak_tr_def] >>
+METIS_TAC []) >>
+`abs_rel r ds_abs1'' \/
+?ds_abs0'. ds_abs0_tr r tau ds_abs0' /\ abs_rel ds_abs0' ds_abs1''` by METIS_TAC [abs1_abs0_weak_simulation] >-
+(Q.EXISTS_TAC `(q,r)` >>
+rw [global_abs0_comb_rel_def, abs0_comb_rel_def, weak_tr_def] >>
+METIS_TAC []) >>
+Q.EXISTS_TAC `(q, ds_abs0')` >>
+rw [global_abs0_comb_rel_def, abs0_comb_rel_def, weak_tr_def] >|
+[DISJ1_TAC >>
+rw [abs0_global_tr_cases] >>
+METIS_TAC [],
+Q.EXISTS_TAC `ds_abs1` >> rw [],
+Q.EXISTS_TAC `ds_abs1''` >> rw []],
+`TX data <> tau /\ RX data <> tau` by rw [] >>
+`?ds_abs1''. (ds_abs1_tr ds_abs1 (TX data) ds_abs1'') /\ (ref_rel ds_abs1'' (dr1', spi1'))` by METIS_TAC [comb_abs1_weak_simulation_lbl_not_tau] >>
+`?ds_abs1'''. (ds_abs1_tr ds_abs1' (RX data) ds_abs1''') /\ (ref_rel ds_abs1''' (dr2', spi2'))` by METIS_TAC [comb_abs1_weak_simulation_lbl_not_tau] >>
+`?ds_abs0'. (ds_abs0_tr q (TX data) ds_abs0') /\ (abs_rel ds_abs0' ds_abs1'')` by METIS_TAC [abs1_abs0_weak_simulation] >>
+`?ds_abs0''. (ds_abs0_tr r (RX data) ds_abs0'') /\ (abs_rel ds_abs0'' ds_abs1''')` by METIS_TAC [abs1_abs0_weak_simulation] >>
+Q.EXISTS_TAC `(ds_abs0',ds_abs0'')` >>
+rw [global_abs0_comb_rel_def, abs0_comb_rel_def, weak_tr_def] >|
+[DISJ1_TAC >>
+rw [abs0_global_tr_cases] >>
+METIS_TAC [],
+Q.EXISTS_TAC `ds_abs1''` >> rw [],
+Q.EXISTS_TAC `ds_abs1'''` >> rw []],
+`TX data <> tau /\ RX data <> tau` by rw [] >>
+`?ds_abs1''. (ds_abs1_tr ds_abs1 (RX data) ds_abs1'') /\ (ref_rel ds_abs1'' (dr1', spi1'))` by METIS_TAC [comb_abs1_weak_simulation_lbl_not_tau] >>
+`?ds_abs1'''. (ds_abs1_tr ds_abs1' (TX data) ds_abs1''') /\ (ref_rel ds_abs1''' (dr2', spi2'))` by METIS_TAC [comb_abs1_weak_simulation_lbl_not_tau] >>
+`?ds_abs0'. (ds_abs0_tr q (RX data) ds_abs0') /\ (abs_rel ds_abs0' ds_abs1'')` by METIS_TAC [abs1_abs0_weak_simulation] >>
+`?ds_abs0''. (ds_abs0_tr r (TX data) ds_abs0'') /\ (abs_rel ds_abs0'' ds_abs1''')` by METIS_TAC [abs1_abs0_weak_simulation] >>
+Q.EXISTS_TAC `(ds_abs0',ds_abs0'')` >>
+rw [global_abs0_comb_rel_def, abs0_comb_rel_def, weak_tr_def] >|
+[DISJ1_TAC >>
+rw [abs0_global_tr_cases] >>
+METIS_TAC [],
+Q.EXISTS_TAC `ds_abs1''` >> rw [],
+Q.EXISTS_TAC `ds_abs1'''` >> rw []],
+`XFER dataI dataO <> tau /\ XFER dataO dataI <> tau` by rw [] >>
+`?ds_abs1''. (ds_abs1_tr ds_abs1 (XFER dataI dataO) ds_abs1'') /\ (ref_rel ds_abs1'' (dr1', spi1'))` by METIS_TAC [comb_abs1_weak_simulation_lbl_not_tau] >>
+`?ds_abs1'''. (ds_abs1_tr ds_abs1' (XFER dataO dataI) ds_abs1''') /\ (ref_rel ds_abs1''' (dr2', spi2'))` by METIS_TAC [comb_abs1_weak_simulation_lbl_not_tau] >>
+`?ds_abs0'. (ds_abs0_tr q (XFER dataI dataO) ds_abs0') /\ (abs_rel ds_abs0' ds_abs1'')` by METIS_TAC [abs1_abs0_weak_simulation] >>
+`?ds_abs0''. (ds_abs0_tr r (XFER dataO dataI) ds_abs0'') /\ (abs_rel ds_abs0'' ds_abs1''')` by METIS_TAC [abs1_abs0_weak_simulation] >>
+Q.EXISTS_TAC `(ds_abs0',ds_abs0'')` >>
+rw [global_abs0_comb_rel_def, abs0_comb_rel_def, weak_tr_def] >|
+[DISJ1_TAC >>
+rw [abs0_global_tr_cases] >>
+METIS_TAC [],
+Q.EXISTS_TAC `ds_abs1''` >> rw [],
+Q.EXISTS_TAC `ds_abs1'''` >> rw []]]);
 
 val _ = export_theory();
